examples/algorithms/qs_seq2.fst
@@ -1,0 +1,138 @@
+module QuickSort.Seq
+open Seq
+
+val count : 'a -> s:seq 'a -> Tot nat (decreases s.length)
+let rec count x s = 
+  if s.length = 0 then 0
+  else if head s = x 
+  then 1 + count x (tail s)
+  else count x (tail s)
+
+let mem x l = count x l > 0
+
+val sorted: ('a -> 'a -> Tot bool) 
+          -> s:seq 'a
+          -> Tot bool (decreases (s.length))
+let rec sorted f s =
+  if s.length <= 1
+  then true
+  else let hd = head s in
+       f hd (index s 1) && sorted f (tail s)
+
+(* Defining a new predicate symbol *)
+type total_order (a:Type) (f: (a -> a -> Tot bool)) =
+    (forall a. f a a)                                           (* reflexivity   *)
+    /\ (forall a1 a2. (f a1 a2 /\ a1<>a2)  <==> not (f a2 a1))  (* anti-symmetry *)
+    /\ (forall a1 a2 a3. f a1 a2 /\ f a2 a3 ==> f a1 a3)        (* transitivity  *)
+
+val swap: a:Type -> s:seq a -> i:nat{i<s.length} -> j:nat{j<s.length} -> Tot (seq a)
+let swap s i j = upd i (index s j) (upd j (index s i) s)
+
+opaque type permutation (a:Type) (s1:seq a) (s2:seq a) =
+       (forall i. count i s1 = count i s2)
+
+assume val lemma_swap_permutes: a:Type -> s:seq a -> i:nat{i<s.length} -> j:nat{j<s.length} -> Lemma (ensures (permutation a s (swap s i j)))
+(* let lemma_swap_permutes s i j = () *)
+
+assume val lemma_count_slice: a:Type -> s:seq a -> i:nat{i<=s.length} -> Lemma 
+         (ensures (forall x. count x s = count x (slice s 0 i) + count x (slice s i s.length)))
+
+assume val partition: f:('a -> 'a -> Tot bool){total_order 'a f}
+    -> s:seq 'a -> pivot:nat{pivot < s.length} -> back:nat{pivot <= back /\ back < s.length} ->
+       Pure (seq 'a * seq 'a)
+         (requires (forall (i:nat{i < s.length}).
+                                 ((i <= pivot ==> f (index s i) (index s pivot))
+                                  /\ (back < i  ==> f (index s pivot) (index s i)))))
+         (ensures (fun res ->
+                     (fun lo hi p ->
+                         (lo.length + hi.length = s.length)
+                      /\ (hi.length > 0)
+                      /\ (index hi 0 = p)
+                      /\ (forall x. (mem x hi ==> f p x)
+                                 /\ (mem x lo ==> not(f p x))
+                                 /\ (count x s = count x hi + count x lo)))
+                     (fst res)
+                     (snd res)
+                     (index s pivot)))
+         (decreases (back - pivot))
+(* let rec partition f s pivot back = *)
+(*   if pivot=back *)
+(*   then (lemma_count_slice s pivot;  *)
+        
+(*         (slice s 0 pivot, slice s pivot s.length)) *)
+(*   else let next = index s (pivot + 1) in *)
+(*        let p = index s pivot in *)
+(*        if f next p *)
+(*        then let s' = swap s pivot (pivot + 1) in  (\* the pivot moves forward *\) *)
+(*             let _ = lemma_swap_permutes s pivot (pivot + 1) in *)
+(*             partition f s' (pivot + 1) back *)
+(*        else let s' = swap s (pivot + 1) back in (\* the back moves backward *\) *)
+(*             let _ = lemma_swap_permutes s (pivot + 1) back in *)
+(*             let res = partition f s' pivot (back - 1) in  *)
+(*             res *)
+
+
+
+val lemma_append_count: a:Type -> lo:seq a -> hi:seq a
+                    -> Lemma (requires True)
+                             (ensures (forall x. count x (append lo hi) = (count x lo + count x hi)))
+                             (decreases (lo.length))
+let rec lemma_append_count lo hi =
+  if lo.length = 0
+  then cut (Eq (Seq.append lo hi) hi)
+  else (cut (Eq (Seq.cons (head lo) (Seq.append (tail lo) hi))
+                (Seq.append lo hi));
+        lemma_append_count (tail lo) hi;
+        let tl_l_h = Seq.append (tail lo) hi in
+        let lh = Seq.cons (head lo) tl_l_h in
+        cut (Eq (tail lh) tl_l_h))
+
+val sorted_concat_lemma: a:Type
+                      -> f:(a -> a -> Tot bool){total_order a f}
+                      -> lo:seq a{sorted f lo}
+                      -> pivot:a
+                      -> hi:seq a{sorted f hi}
+                      -> Lemma (requires (forall y. (mem y lo ==> not(f pivot y))
+                                                 /\ (mem y hi ==> f pivot y)))
+                               (ensures (sorted f (append lo (cons pivot hi))))
+                               (decreases (lo.length))
+                               (* [SMTPat  (sorted f (append lo (pivot::hi)))] *)
+let rec sorted_concat_lemma f lo pivot hi =
+  if lo.length = 0
+  then (cut (Eq (append lo (cons pivot hi)) (cons pivot hi));
+        cut (Eq (tail (cons pivot hi)) hi))
+  else (sorted_concat_lemma f (tail lo) pivot hi;
+        Seq.lemma_append_cons lo (cons pivot hi);
+        Seq.lemma_tl (head lo) (append (tail lo) (cons pivot hi)))
+        
+
+
+val cons_perm: a:Type -> tl:seq a -> s:seq a{length s > 0} ->
+         Lemma (requires (permutation a tl (tail s)))
+               (ensures (permutation a (cons (head s) tl) s))
+let cons_perm tl s = Seq.lemma_tl (head s) tl
+
+
+val sort: f:('a -> 'a -> Tot bool){total_order 'a f}
+       -> s1:seq 'a
+       -> Tot (s2:seq 'a{sorted f s2 /\ permutation 'a s1 s2})
+              (decreases (s1.length))
+let rec sort f s =
+  if s.length <= 1 then s
+  else let lo, hi = partition f s 0 (s.length - 1) in
+       let pivot = head hi in
+
+       let hi_tl = tail hi in
+       let l = sort f lo in
+       let h = sort f hi_tl in
+
+       let result = Seq.append l (cons pivot h) in
+
+       sorted_concat_lemma f l pivot h;
+       lemma_append_count l (cons pivot h);
+       cons_perm h hi;
+
+       result
+
+
+
